Defined new simulation, before retring the global simulation

concur/CallconvNew.v
@@ -8,6 +8,245 @@ Require Import CKLR.
 Require Import LanguageInterface.
 Require Import Smallstep.
 
+(* Require Import RelationClasses. *)
+Class Lens (T A: Type) :=
+  {
+    get : T -> A;
+    set : T -> A -> T;
+    get_set : forall t a, get (set t a) = a;
+    set_get : forall t, set t (get t) = t;
+    set_set : forall t a1 a2, set (set t a1) a2 = set t a2;
+  }.
+
+Program Instance lens_id {T: Type} : Lens T T :=
+  {
+    get t := t;
+    set _ t := t;
+  }.
+
+Program Instance lens_fst {U V} : Lens (U * V) U :=
+  {
+    get '(u, v) := u;
+    set '(_, v) u := (u, v);
+  }.
+
+Program Instance lens_snd {U V} : Lens (U * V) V :=
+  {
+    get '(u, v) := v;
+    set '(u, _) v := (u, v);
+  }.
+
+Class World (T: Type) :=
+  {
+    w_state : Type;
+    w_lens : Lens T w_state;
+    w_acc : w_state -> w_state -> Prop;
+    w_acc_trans : PreOrder  w_acc;
+  }.
+
+Existing Instance w_lens.
+Existing Instance w_acc_trans.
+Arguments w_state {_} _.
+Arguments w_acc {_ _}.
+Infix "*->" := w_acc (at level 60, no associativity).
+
+Module GS.
+
+  Record callconv {li1 li2} :=
+  mk_callconv {
+    ccworld : Type;
+    ccworld_world : World ccworld;
+    match_senv: ccworld -> Genv.symtbl -> Genv.symtbl -> Prop;
+    match_query: ccworld -> query li1 -> query li2 -> Prop;
+    match_reply: ccworld -> reply li1 -> reply li2 -> Prop;
+
+    match_senv_public_preserved:
+      forall w se1 se2,
+        match_senv w se1 se2 ->
+        forall id, Genv.public_symbol se2 id = Genv.public_symbol se1 id;
+    match_senv_valid_for:
+      forall w se1 se2 sk,
+        match_senv w se1 se2 ->
+        Genv.valid_for sk se1 ->
+        Genv.valid_for sk se2;
+    }.
+
+  Arguments callconv: clear implicits.
+  (* Existing Instance ccworld_world | 3. *)
+  
+  Definition gworld {li1 li2}(cc: callconv li1 li2) := w_state (ccworld_world cc).
+  
+Section FSIM.
+
+    Context {li1 li2} (cc: callconv li1 li2).
+    Context (se1 se2: Genv.symtbl).
+    Context (wb: ccworld cc).
+    Context {state1 state2: Type}.
+
+    Let gw_type := gworld cc.
+    
+    Record fsim_properties
+           (L1: lts li1 li1 state1) (L2: lts li2 li2 state2)
+           (index: Type) (order: index -> index -> Prop)
+           (match_states: gw_type -> index -> state1 -> state2 -> Prop) :=
+      {
+        fsim_match_initial_states:
+          forall q1 q2 s1, match_query cc wb q1 q2 -> initial_state L1 q1 s1 ->
+          match_senv cc wb se1 se2 ->
+          exists i, exists s2, initial_state L2 q2 s2 /\ match_states (get wb) i s1 s2;
+        fsim_match_final_states:
+          forall gw i s1 s2 r1, match_states gw i s1 s2 -> final_state L1 s1 r1 ->
+          exists r2, final_state L2 s2 r2 /\
+          match_reply cc (set wb gw) r1 r2;
+        fsim_match_external:
+          forall gw i s1 s2 q1, match_states gw i s1 s2 -> at_external L1 s1 q1 ->
+          exists wa q2 , at_external L2 s2 q2 /\ exists gw', gw *-> gw' /\ get wa = gw' /\
+          match_query cc wa q1 q2 /\ match_senv cc wa se1 se2 /\
+          forall r1 r2 s1' gw'', gw' *-> gw'' -> match_reply cc (set wa gw'') r1 r2 ->
+          after_external L1 s1 r1 s1' ->
+          exists i' s2', after_external L2 s2 r2 s2' /\
+          exists gw''' , gw'' *-> gw''' /\ match_states gw''' i' s1' s2';
+        fsim_simulation:
+          forall s1 t s1', Step L1 s1 t s1' ->
+          forall gw i s2, match_states gw i s1 s2 ->
+          exists i', exists s2', (Plus L2 s2 t s2' \/ (Star L2 s2 t s2' /\ order i' i)) /\
+          exists gw', gw *-> gw' /\ match_states gw' i' s1' s2';
+      }.
+    Arguments fsim_properties : clear implicits.
+
+    Lemma fsim_simulation':
+      forall L1 L2 index order match_states, fsim_properties L1 L2 index order match_states ->
+      forall i s1 t s1', Step L1 s1 t s1' ->
+      forall gw s2, match_states gw i s1 s2 ->
+      exists i' gw', gw *-> gw' /\
+      ((exists s2', Plus L2 s2 t s2' /\ match_states gw' i' s1' s2')
+      \/ (order i' i /\ t = E0 /\ match_states gw' i' s1' s2)).
+    Proof.
+      intros. exploit @fsim_simulation; eauto.
+      intros (i' & s2' & A & wi & Hi & B).
+      exists i', wi. repeat split; eauto.
+      destruct A.
+      left; exists s2'; auto.
+      destruct H2. inv H2.
+      right; eauto.
+      left; exists s2'; split; auto. econstructor; eauto.
+    Qed.
+
+    Section SIMULATION_SEQUENCES.
+
+      Context L1 L2 index order match_states
+              (S: fsim_properties L1 L2 index order match_states).
+
+      Lemma simulation_star:
+        forall s1 t s1', Star L1 s1 t s1' ->
+        forall gw i s2, match_states gw i s1 s2 ->
+        exists gw' i', exists s2', Star L2 s2 t s2' /\
+        gw *-> gw'  /\ match_states gw' i' s1' s2'.
+      Proof.
+        induction 1; intros.
+        eexists _, i; exists s2; repeat split; auto. apply star_refl.
+        reflexivity. assumption.
+        exploit fsim_simulation; eauto.
+        intros (i' & s2' & A & wi & Hi & B).
+        exploit IHstar; eauto.
+        intros (wj & i'' & s2'' & Hx & Hj & C).
+        exists wj, i''; exists s2''; repeat split; auto.
+        eapply star_trans; eauto.
+        intuition auto. apply plus_star; auto.
+        all: etransitivity; eauto.
+      Qed.
+
+      
+    End SIMULATION_SEQUENCES.
+  End FSIM.
+
+  Arguments fsim_properties  {_ _} _ _ _ _  {_ _} L1 L2 index order match_states.
+
+  Record fsim_components {li1 li2} (cc: callconv li1 li2) L1 L2 :=
+    Forward_simulation {
+        fsim_index: Type;
+        fsim_order: fsim_index -> fsim_index -> Prop;
+        fsim_match_states: _;
+
+        fsim_skel: skel L1 = skel L2;
+        fsim_lts se1 se2 w:
+          GS.match_senv cc w se1 se2 ->
+          Genv.valid_for (skel L1) se1 ->
+          fsim_properties cc se1 se2 w (activate L1 se1) (activate L2 se2)
+            fsim_index fsim_order (fsim_match_states se1 se2 w);
+        fsim_order_wf:
+          well_founded fsim_order;
+      }.
+
+  Arguments Forward_simulation {_ _ cc L1 L2 fsim_index}.
+
+  Definition forward_simulation {li1 li2} cc L1 L2 :=
+    inhabited (@fsim_components li1 li2 cc L1 L2).
+  
+  Arguments Forward_simulation {_ _ cc L1 L2 fsim_index}.
+
+End GS.
+
+(** Definition of new CAinjp *)
+Require Import Conventions Mach Asm.
+Require Import InjectFootprint CA.
+
+Definition get_injp := cajw_injp.
+
+Definition set_injp (wa: cc_cainjp_world) (w : injp_world) :=
+  match wa with cajw w' sig rs => cajw w sig rs end.
+
+Program Instance lens_injp : Lens (cc_cainjp_world) injp_world :=
+  {
+    get := get_injp;
+    set := set_injp;
+  }.
+Next Obligation. destruct t. reflexivity. Qed.
+Next Obligation. destruct t. reflexivity. Qed.
+Next Obligation. destruct t. reflexivity. Qed.
+
+Program Instance CAworld : World cc_cainjp_world :=
+    {
+      w_state := injp_world;
+      w_lens := lens_injp;
+      w_acc := injp_acc;
+      w_acc_trans := injp_acc_preo;
+    }.
+     
+Inductive cc_c_asm_injp_mr : cc_cainjp_world -> c_reply -> reply li_asm -> Prop :=
+  cc_c_asm_injp_mr_intro sg res  j' m' tm' Hm' (rs rs' :regset) :
+     let tres := rs_getpair (map_rpair preg_of (loc_result sg)) rs' in
+     Val.inject j' res tres ->
+     (forall r, is_callee_save r = true -> rs' (preg_of r) = rs (preg_of r)) ->
+     (*(forall b ofs, loc_init_args (size_arguments sg) tsp b ofs ->
+              loc_out_of_reach j m b ofs) -> *)
+     rs'#SP = rs#SP -> rs'#PC = rs#RA ->
+     cc_c_asm_injp_mr
+       (cajw (injpw j' m' tm' Hm') sg rs)
+       (cr res m')
+       (rs', tm').
+
+Program Definition cc_c_asm_injp_new : GS.callconv li_c li_asm :=
+  {|
+    GS.ccworld := cc_cainjp_world;
+    GS.ccworld_world := CAworld;
+    GS.match_senv w := match_stbls injp (cajw_injp w);
+    GS.match_query := cc_c_asm_injp_mq;
+    GS.match_reply := cc_c_asm_injp_mr
+  |}.
+Next Obligation.
+  inv H. inv H1. eauto.
+Qed.
+Next Obligation.
+  inv H.
+  eapply Genv.valid_for_match in H2.
+  apply H2. eauto.
+Qed.
+
+
+
+(** Legacy  * )
+(*
 Record callconvnew {li1 li2} :=
   mk_callconv {
     ccworld : Type;
@@ -142,3 +381,5 @@ Next Obligation.
   apply H2. eauto.
 Qed.
 Next Obligation.
+ *)
+*)
